experimental/ni_coq/vfiles/PossibilisticNI.v
@@ -7,6 +7,9 @@ From OakIFC Require Import
     Events
     LowEquivalences
     TraceTheorems.
+From mathcomp Require Import all_ssreflect finmap.
+From RecordUpdate Require Import RecordSet.
+Import RecordSetNotations.
 
 
 (*
@@ -66,16 +69,100 @@ Definition conjecture_possibilistic_ni := forall ell t1_init t2_init t1n,
         (step_system_ev_multi t2_init t2n) /\
         (trace_low_eq ell t1n t2n)).
 
+Theorem possibilistic_ni_1step_node: forall ell id t1 t2 s1 s2 n1 n2 t1',
+    (head_st t1 = Some s1) ->
+    (head_st t2 = Some s2) ->
+    (s1.(nodes) .[?id] = Some n1) ->
+    (s2.(nodes) .[?id] = Some n2) ->
+    (trace_low_eq ell t1 t2) ->
+    (step_node_ev id (ncall n1) t1 t1') ->
+    (exists t2',
+        (step_node_ev id (ncall n2) t2 t2') /\
+        (trace_low_eq ell t1' t2')).
+Proof.
+Admitted. (* WIP *)
+
+Theorem call_havoc_unwind: forall ell id c t1 t2 t1' t2',
+    (trace_low_eq ell t1 t2) ->
+    (t1' = head_set_call t1 id c) ->
+    (t2' = head_set_call t2 id c) ->
+    (trace_low_eq ell t1' t2').
+Proof.
+Admitted. (* WIP *)
+
+Theorem trace_loweq_to_deref_node: forall ell t1 t2 id s1 n1,
+(* If two traces are low-equivalent and in the first trace:
+    - the head element has some state (it's not an emty trace)
+    - and in the head state, id can be dereferenced to some node
+    then:
+    - there must be some head state in the other trace (s2)
+    - and we must be able to also dereference id in s2 to some node 
+Mostly, this is just a consequence of the def of trace-low-equivalence.
+*)
+    (trace_low_eq ell t1 t2) ->
+    (head_st t1 = Some s1) ->
+    ((nodes s1).[? id] = Some n1) ->
+    (exists s2 n2,
+        head_st t2 = Some s2 /\ 
+        (nodes s2).[? id] = Some n2 ).
+Proof.
+    intros.
+    destruct (head_st t2) eqn:Ht2head.
+    - (* some s *)
+        destruct (nodes s).[? id] eqn:Hsid.
+            + (* some n *)
+                exists s. exists n.
+                split; (reflexivity || assumption).
+            + (* none *)
+                inversion H; subst.
+                * (* t1 = [] and t2 = [] *) discriminate H0.
+                * exfalso. inversion H4; subst. simpl in Ht2head.
+                 unfold node_state_low_eq in H5.
+                 inversion Ht2head. rewrite H8 in H5. specialize (H5 id).
+                 rewrite Hsid in H5. simpl in H0. inversion H0.
+                 rewrite H9 in H5. rewrite H1 in H5. assumption.
+    - (* none *)
+        inversion H; subst. 
+            + discriminate H0.
+            + inversion Ht2head.
+Qed.
+ 
 Theorem possibilistic_ni_1step: forall ell t1 t2 t1',
     (trace_low_eq ell t1 t2) ->
     (step_system_ev t1 t1') ->
     (exists t2',
         (step_system_ev t2 t2') /\
         (trace_low_eq ell t1' t2')).
-Admitted. (* NOTE: work in progress *)
+Proof.
+    intros.
+    inversion H0; subst.
+    rename t' into t1_sn. rename s into s1. rename s' into s1'. rename n into n1.
+    specialize (trace_loweq_to_deref_node ell t1 t2 id s1 n1
+        H H1 H3) as [s2 [n2 [Ht2s2 Hs2n2]]].
+    specialize (possibilistic_ni_1step_node ell id
+        t1 t2 s1 s2 n1 n2 t1_sn  H1 Ht2s2 H3 Hs2n2 H H5)
+            as [t2_sn [Hnstep2 Hnstep_leq]].
+    assert (Hs2': exists s2', head_st t2_sn = Some s2'). {
+        (* this assertion is essentially re-stating node_no_steps_to_empty
+        in a way that gives us a particular head state of t2_sn *)
+        destruct t2_sn; subst.
+        - exfalso. apply (node_no_steps_to_empty t2 id (ncall n2)). assumption.
+        - exists (fst p). simpl. destruct p. reflexivity.
+    }
+    destruct Hs2' as [s2' Hs2']. 
+    remember (head_set_call t2_sn id c') as t2'.
+    exists t2'. split.
+    +  (* can step from t2_sn to t2' *)
+        subst. apply (ValidStep id n2 (ncall n2) c' s2 t2 s2' t2_sn);
+            (assumption || reflexivity).
+    + (* low-equiv t1' t2' *)
+        remember (head_set_call t1_sn id c') as t1' eqn:Ht1'.
+        apply (call_havoc_unwind ell id c' t1_sn t2_sn t1' t2');
+            (assumption || reflexivity).
+Qed. 
 
-
-Theorem possibilistic_ni: conjecture_possibilistic_ni. Proof.
+Theorem possibilistic_ni: conjecture_possibilistic_ni.
+Proof.
 unfold conjecture_possibilistic_ni.
 intros ell t1_init t2_init t1n [Hinit_tleq [Ht1_init [Ht2_init Ht1_mstep_t1n]]].
 remember ([]: trace) as emp eqn:R.
@@ -84,31 +171,19 @@ induction t1n.
         exfalso. apply (no_steps_to_empty t1_init Ht1_mstep_t1n).
     - (* inductive case *)
     inversion Ht1_mstep_t1n ; subst.
-        + assert (E: exists t2n,
-            (step_system_ev t2_init t2n) /\
-            (trace_low_eq ell (a::t1n) t2n)) by
-            apply (possibilistic_ni_1step ell t1_init t2_init
-                (a::t1n) Hinit_tleq H).
-            destruct E as [t2n [E1 E2]].
+        + specialize (possibilistic_ni_1step ell t1_init t2_init
+            (a::t1n) Hinit_tleq H) as [t2n [E1 E2]].
             exists t2n. split. constructor. assumption. assumption.
         + rename Ht1_mstep_t1n into Ht1_mstep_at1n.
-        assert (E: step_system_ev_multi t2 t1n)
-            by apply (step_system_multi_backwards t2 t1n a H0).
+        specialize (step_system_multi_backwards t2 t1n a H0) as E.
         assert (H': step_system_ev_multi t1_init t2) by
             (constructor; assumption).
-        assert (Ht1_mstep_t1n: step_system_ev_multi t1_init t1n)
-            by apply (step_system_transitive t1_init t2 t1n H' E).
-        apply IHt1n in Ht1_mstep_t1n as [t2n [Hm_t2_init_t2n Hleq_t1n_t2n]].
-        assert (E2: step_system_ev t1n (a::t1n))
-            by apply (step_system_multi_extends t2 t1n a H0).
-            (*need to get non-multi from E2.  *)
-        assert (E3: exists t2n',
-            (step_system_ev t2n t2n') /\
-            (trace_low_eq ell (a::t1n) t2n')) by
-            apply (possibilistic_ni_1step ell t1n t2n (a::t1n) Hleq_t1n_t2n E2).
-            destruct E3 as [t2n' [Hs_t2n_t2n' Hleq_at1n_t2n']].
-        exists t2n'.
-        split.
-        + apply (step_system_transitive t2_init t2n t2n'). assumption.
+        specialize (IHt1n (step_system_transitive t1_init t2 t1n H' E))
+            as [t2n [Hm_t2_init_t2n Hleq_t1n_t2n]].
+        specialize (step_system_multi_extends t2 t1n a H0) as E2.
+        specialize (possibilistic_ni_1step ell t1n t2n (a::t1n) Hleq_t1n_t2n E2)
+            as [t2n' [Hs_t2n_t2n' Hleq_at1n_t2n']].
+        exists t2n'. split.
+        apply (step_system_transitive t2_init t2n t2n'). assumption.
         constructor. assumption. assumption.
 Qed.
